

Homeworks of Bayesian Inference

(B004652)

Giovanni Papini

Last revision October 2, 2018

Week 1

Exchangeability and stochastic processes

1.1 Exercise 1

1.1.1 Data

- E_1, E_2, E_3, E_4, E_5 , events of simple alternative, exchangeable
- $P(E_2) = \omega_1 = \frac{1}{2}$
- $P(E_3 \wedge E_5) = \omega_2 = \frac{1}{4}$
- $\omega_5 = \frac{\omega_3^5}{\binom{5}{3}} = \frac{\omega_1^5}{\binom{5}{1}} = \frac{1}{30}$

1.1.2 Questions

Compute:

1. $P(E_2 \wedge E_3 \wedge E_4) = \omega_3$
2. $P(E_1 \wedge E_2 \wedge E_3 \wedge E_4) = \omega_4$
3. $P(E_1 \wedge E_2 \wedge \bar{E}_3 \wedge \bar{E}_4 \wedge \bar{E}_5) = \frac{\omega_2^5}{\binom{5}{2}}$

1.1.3 Solutions

First we find ω_1^5 and ω_3^5 :

$$\omega_1^5 = \frac{1}{30} \cdot \binom{5}{1} = \frac{1}{6}$$
$$\omega_3^5 = \frac{1}{30} \cdot \binom{5}{3} = \frac{1}{3}$$

Knowing that

$$\omega_h = \frac{1}{\binom{n}{h}} \sum_{r=h}^n \omega_r^n \binom{r}{h}$$

we can write that

$$\begin{aligned}
 \omega_1 &= \frac{\omega_1^5(1) + \omega_2^5(2) + \omega_3^5(3) + \omega_4^5(4) + \omega_5^5(5)}{\binom{5}{1}} \\
 &= \frac{1}{6} \cdot \frac{1}{5} + \frac{2}{5} \omega_2^5 + \frac{1}{5} \cdot \frac{1}{3} \cdot 3 + \frac{1}{5} \cdot 4 \omega_4^5 + \frac{1}{30} \\
 &= \frac{8}{30} + \frac{2}{5} \omega_2^5 + \frac{4}{5} \omega_4^5 \\
 \\
 \omega_2 &= \frac{\omega_2^5(2) + \omega_3^5(3) + \omega_4^5(4) + \omega_5^5(5)}{\binom{5}{2}} \\
 &= \frac{1}{10} \omega_2^5 + \frac{1}{10} \cdot \frac{1}{10} \cdot 3 + \frac{1}{10} \cdot 6 \omega_4^5 + \frac{1}{30} \\
 &= \frac{2}{15} + \frac{1}{10} \omega_2^5 + \frac{3}{5} \omega_4^5
 \end{aligned}$$

Combining them:

$$\begin{aligned}
 &\begin{cases} \frac{2}{5} \omega_2^5 + \frac{4}{5} \omega_4^5 = \frac{1}{2} - \frac{8}{30} \\ \frac{1}{10} \omega_2^5 + \frac{3}{5} \omega_4^5 = \frac{1}{4} - \frac{2}{15} \end{cases} \\
 \implies &\begin{cases} \omega_2^5 = \frac{7}{24} \\ \omega_4^5 = \frac{7}{48} \end{cases}
 \end{aligned}$$

Now we can obtain

$$\begin{aligned}
 \omega_3 &= \frac{\omega_3^5(3) + \omega_4^5(4) + \omega_5^5(5)}{\binom{5}{3}} = \frac{1}{3} \cdot \frac{1}{10} + \frac{7}{48} \cdot 4 \cdot \frac{1}{10} + \frac{1}{30} = \frac{1}{8} \\
 \omega_4 &= \frac{\omega_4^5(4) + \omega_5^5(5)}{\binom{5}{4}} = \frac{7}{48} \cdot \frac{1}{5} + \frac{1}{30} = \frac{1}{16}
 \end{aligned}$$

1.2 Exercise 2

1.2.1 Data

- Process of simple alternative $\{|E_n|\}$
- $P(E_1) = \omega_1 = \frac{1}{2}$
- $P(E_1 \wedge E_2) = \omega_2 = \frac{1}{4}$
- $P(E_1 \wedge E_2 \wedge E_3) = \omega_3 = \frac{1}{7}$
- $P(E_1 \wedge E_2 \wedge E_3 \wedge E_4) = \frac{3}{28}$

1.2.2 Questions

1. Could the 4 indicators $|E_1|$, $|E_2|$, $|E_3|$ and $|E_4|$ be the starting path of an exchangeable process?
2. Could it continue for at least one step?

1.2.3 Solutions

1. An exchangeable process must satisfy the condition

$$(-1)^{n-h} \Delta^{n-h} \omega_h \geq 0, \forall n, h \leq n$$

Thus we compute

- $(-1)^{4-1} \Delta^{4-1} \omega_1 = (-1) \cdot \Delta^3 \omega_1 = \frac{1}{14} \geq 0$
- $(-1)^{4-2} \Delta^{4-2} \omega_2 = (-1) \cdot \Delta^2 \omega_2 = \frac{1}{14} \geq 0$
- $(-1)^{4-3} \Delta^{4-3} \omega_3 = (-1) \cdot \Delta \omega_3 = \frac{1}{28} \geq 0$
- $(-1)^{4-4} \Delta^{4-4} \omega_4 = (-1) \cdot \omega_4 = \frac{3}{28} \geq 0$

Thus we can affirm that the process is exchangeable.

- 2.

Week 2

Conjugate priors and posterior distributions

2.1 Exercise 2.3

2.1.1 Data

- $p(x, y, z) \propto f(x, z) g(y, z) h(z)$

2.1.2 Questions

Prove that:

1. $p(x|y, z) \propto f(x, z)$
2. $p(y|x, z) \propto g(y, z)$
3. X and Y conditionally independent, given Z .

2.1.3 Solutions

We know by definition that

$$p(x|y, z) = \frac{p(x, y, z)}{p(y, z)}$$

and also that

$$p(y, z) = \int_{S_X} p(x, y, z) \partial x \propto \int_{S_X} f(x, z) g(y, z) h(z) \partial x = g(y, z) h(z) \int_{S_X} f(x, z) \partial x$$

Where S_X is the support of the r.v. X . Then we can write

$$\begin{aligned} p(x|y, z) &= \frac{f(x, z) g(y, z) h(z)}{g(y, z) h(z) \int_{S_X} f(x, z) \partial x} \\ &= \frac{f(x, z)}{\int_{S_X} f(x, z) \partial x} \end{aligned}$$

But $\int_{S_X} f(x, z) \partial x$ is constant given z , so we can say

$$p(x|y, z) \propto f(x, z)$$

as we wanted to show.

Similarly, we can write

$$\begin{aligned} p(y|x, z) &= \frac{p(x, y, z)}{p(x, z)} \\ &= \frac{f(x, z)g(y, z)h(z)}{f(x, z)h(z) \int_{S_Y} g(y, z) \partial y} \\ &= \frac{g(y, z)}{\int_{S_Y} g(y, z) \partial y} \\ &\propto g(y, z) \end{aligned}$$

To show that $X \perp Y$ given Z we have to prove that $p(y|z, x) = p(y|z)$, so:

$$\begin{aligned} p(y|z) &= \frac{p(y, z)}{p(z)} \\ &= \frac{\int_{S_X} f(x, z)g(y, z)h(z) \partial x}{\int_{S_X} \int_{S_Y} f(x, z)g(y, z)h(z) \partial y \partial x} \\ &= \frac{g(y, z)h(z) \int_{S_X} f(x, z) \partial x}{h(z) \int_{S_X} f(x, z) \partial x \int_{S_Y} g(y, z) \partial y} \\ &= \frac{g(y, z)}{\int_{S_Y} g(y, z) \partial y} \\ &= p(y|x, z) \end{aligned}$$

2.2 Exercise 3.5

2.2.1 Data

- $p(y|\phi) = c(\phi)h(y) \exp(\phi t(y))$
- $p_1(\theta) \dots p_k(\theta)$ conjugate priors
- $\tilde{p}(\theta) = \sum_{k=1}^K \omega_k p_k(\theta)$ where $\omega_k > 0$ and $\sum_k \omega_k = 1$

2.2.2 Questions

1. $p(\theta|y)$ as a function of $p(y|\theta)$ and \tilde{p}
2. Previous question but in the case that $\theta \sim \text{Pois}$ and $p_1 \dots p_k \sim \Gamma$

2.2.3 Solution

For the Bayes rule:

$$p(\theta|y) \propto p(y|\theta) \cdot p(\theta) = p(y|\theta) \cdot \tilde{p}(\theta)$$

In the particular case that it's the sample comes from a Poisson distribution and the prior is a mixture of Gamma distributions:

$$\begin{aligned} p(\theta|y) &\propto p(y|\theta) \cdot \tilde{p}(\theta) \\ &\propto \theta^k \exp(\theta) \sum_k w_k x^{\alpha_k-1} \exp\left(-\frac{x}{\beta_k}\right) \end{aligned}$$